\documentclass[10pt]{article}
\usepackage{fontspec}
\setmainfont{IBM Plex Sans}
\usepackage{amsmath, amssymb}
\usepackage{geometry}
\geometry{a4paper, margin=0.3in}
\usepackage{mathtools}
\usepackage{lscape}
\usepackage{graphicx}
\usepackage{enumitem}
\usepackage{mathabx}

\title{DER Models}
\author{Seohyun Jang}

\begin{document}

\maketitle

\section{Without Storage}
\subsection{Disaggregation}
\begin{subequations}
\begin{align}
    \text{max} \quad & \sum_{t\in T}\left(P_t^{DA}x_{it} + \mathbb{E}\left[P_t^{RT}(\xi)y_{it}^{+}(\xi) - P_t^{PN}y_{it}^{-}(\xi)\right]\right) &\\
    \text{s.t.} \quad & R_{it}(\xi) - x_{it} = y_{it}^{+}(\xi) - y_{it}^{-}(\xi) \quad  \forall t \in T &\\
    & R_{it}(\xi) \geq y^+_{it}(\xi) \quad \forall t \in T &\\
    & y_{it}^{+}(\xi) \leq M z_{it}(\xi), \quad y_{it}^{-}(\xi) \leq M (1 - z_{it}(\xi)) \quad \forall t \in T &\\
    & x_{it}^{DA} \geq 0, y_{it}^{+}(\xi) \geq 0, y_{it}^{-}(\xi) \geq 0, z_{it}(\xi) \in \{0, 1\} \quad \forall t \in T
\end{align}
\end{subequations}

\subsection{Aggregation}
\begin{subequations}
\begin{align}
    \text{max} \quad &\sum_{t\in T}\left(P_t^{DA}\alpha_{t} + \mathbb{E}\left[P_t^{RT}(\xi)\beta_{t}^{+}(\xi) - P_t^{PN}\beta_{t}^{-}(\xi)\right]\right) &\\
    \text{s.t.} \quad &\sum_{i\in I}R_{it}(\xi) - \alpha_{t} = \beta_{t}^{+}(\xi) - \beta_{t}^{-}(\xi) \quad \forall t \in T &\\
    & \sum_{i\in I}R_{it}(\xi) \geq \beta^+_{t}(\xi) \quad \forall t \in T &\\
    & \beta_{t}^{+}(\xi) \leq M z_{t}(\xi), \quad \beta_{t}^{-}(\xi) \leq M (1 - z_{t}(\xi)) \quad \forall t\in T &\\
    & \alpha_{t}^{DA} \geq 0, \beta_{t}^{+}(\xi) \geq 0, \beta_{t}^{-}(\xi) \geq 0, z_{t}(\xi) \in \{0, 1\} \quad \forall t\in T 
\end{align}
\end{subequations}

\subsection{Settlement}
\begin{subequations}
\begin{align}
    \text{max} \quad &\sum_{t\in T}\left(P_t^{DA}\alpha_t + \mathbb{E}\left[P_t^{RT}(\xi)\beta^+_{t}(\xi) - P_t^{PN}\beta^-_{t}(\xi)\right]\right) &\\
    \text{s.t.} \quad &\sum_{i\in I}R_{it}(\xi) - \alpha_{t}^{DA} = \beta_{t}^{+}(\xi) - \beta_{t}^{-}(\xi) \quad \forall t \in T &\\
    & \sum_{i\in I}R_{it}(\xi) \geq \beta^+_{t}(\xi) \quad \forall t \in T &\\
    & \beta_{t}^{+}(\xi) \leq M z_{t}(\xi), \quad \beta_{t}^{-}(\xi) \leq M (1 - z_{t}(\xi)) \quad \forall t\in T &\\
    & \alpha_t = \sum_{i \in I} x_{it}(\xi), \quad \beta^+_{t}(\xi) = \sum_{i \in I} e^+_{it}(\xi), \quad \beta^-_{t}(\xi) = \sum_{i \in I} e^-_{it}(\xi) \quad \forall t \in T &\\
    & R_{it}(\xi) - x_{it}(\xi) = y_{it}^{+}(\xi) - y_{it}^{-}(\xi) \quad  \forall t \in T &\\
    & R_{it}(\xi) \geq y^+_{it}(\xi) \quad \forall t \in T &\\
    & y_{it}^{+}(\xi) \leq M z_{it}(\xi), \quad y_{it}^{-}(\xi) \leq M (1 - z_{it}(\xi)) \quad \forall t \in T &\\
    & \sum_{j \in I, j \neq i} d_{ijt}(\xi) \leq y^+_{it}(\xi), \quad \sum_{j \in I, j \neq i} d_{jit}(\xi) \leq y^-_{it}(\xi) \quad \forall t \in T &\\
    & d_{iit}(\xi) = 0 \quad \forall t \in T &\\
    & e^+_{it}(\xi) = y^+_{it}(\xi) - \sum_{j \in I, j \neq i} d_{ijt}(\xi) \quad \forall t \in T &\\
    & e^-_{it}(\xi) = y^-_{it}(\xi) - \sum_{j \in I, j \neq i} d_{jit}(\xi) \quad \forall t \in T 
\end{align}
\end{subequations}

\newpage
\section{With Storage}

\subsection{Disaggregation}
\begin{subequations}
    \begin{align}
    \text{max} \quad &\sum_{t\in T}\left(P_t^{DA}x_{it} + \mathbb{E}\left[P_t^{RT}(\xi)y_{it}^{+}(\xi) - P_t^{PN}y_{it}^{-}(\xi)\right]\right)&\\    
    \text{s.t.} \quad &R_{it}(\xi) - x_{it} = y_{it}^{+}(\xi) - y_{it}^{-}(\xi) + z^C_{it}(\xi) - z^D_{it}(\xi)\quad  \forall i, t &\\ 
    &R_{it}(\xi) \geq y^+_{it}(\xi) \quad \forall i ,t &\\
    &z_{i,t+1}(\xi) = z_{it}(\xi) + z^C_{it}(\xi) - z^D_{it}(\xi) \quad \forall i, t &\\
    &z^D_{it}(\xi) \le z_{it}(\xi) \quad \forall i, t &\\
    &z^C_{it}(\xi) \le K_i-z_{it}(\xi) \quad \forall i, t &\\
    &0 \leq z_{it}(\xi) \leq K_i \quad \forall i, t &\\
    &y^+_{it}(\xi) \leq M_1 \rho_{it}(\xi), \quad y^-_{it}(\xi) \leq M_1 (1 - \rho_{it}(\xi)) \quad \forall i, t &\\
    &y^-_{it}(\xi) \leq M_1 \delta_{it}(\xi), \quad z^C_{it}(\xi) \leq M_1 (1 - \delta_{it}(\xi)) \quad \forall i, t &\\
    &z^C_{it}(\xi) \leq M_1 \zeta_{it}(\xi), \quad z^D_{it}(\xi) \leq M_1 (1 - \zeta_{it}(\xi)) \quad \forall i, t &
    \end{align}
\end{subequations}

\subsection{Aggregation}
\begin{subequations}
    \begin{align}
    \text{max} \quad &\sum_{t\in T}\left(P_t^{DA}\alpha_t + \mathbb{E}\left[P_t^{RT}(\xi)\beta_{t}^{+}(\xi) - P_t^{PN}\beta_{t}^{-}(\xi))\right]\right)&\\   
    \text{s.t.} \quad & \sum_{i \in I} R_{it}(\xi) - \alpha_t = \beta^+_t(\xi) - \beta^-_t(\xi) + \gamma^C_t(\xi) - \gamma^D_t(\xi) \quad \forall t &\\
    &\sum_{i\in I}R_{it}(\xi) \geq \beta_{t}^{+}(\xi) \quad \forall t &\\ 
    &\gamma^D_t(\xi) \le \gamma_{t}(\xi) \quad \forall t &\\
    &\gamma^C_t(\xi) \le \sum_{i \in I}K_i - \gamma_{t}(\xi) \quad \forall t &\\
    &0 \leq \gamma_t(\xi) \leq \sum_{i \in I} K_i \quad \forall t &\\
    &\gamma_{t+1}(\xi) = \gamma_{t}(\xi) + \gamma^C_t(\xi) - \gamma^D_t(\xi) \quad \forall t &\\
    &\beta^+_t(\xi) \le M_2 \mu_t(\xi), \quad \beta^-_t(\xi) \le M_2 (1 - \mu_t(\xi)) \quad \forall t &\\ 
    &\beta^-_t(\xi) \le M_2 \eta_t(\xi), \quad \gamma^C_t(\xi) \le M_2 (1 - \eta_t(\xi)) \quad \forall t &\\
    &\gamma^C_t(\xi) \le M_2\lambda_t(\xi), \quad \gamma^D_t(\xi) \le M_2(1 - \lambda_t(\xi)) \quad \forall t &
    \end{align}
\end{subequations}

\subsection{Settlement}
\begin{subequations}
    \small
    \begin{align*}
    \text{max} \quad &\sum_{t\in T}\left(P_t^{DA}\alpha_t + \mathbb{E}\left[P_t^{RT}(\xi)\beta_{t}^{+}(\xi) - P_t^{PN}\beta_{t}^{-}(\xi))\right]\right)&\\   
    &&\\
    \text{s.t.} \quad &R_{it}(\xi) - x_{it} = y_{it}^{+}(\xi) - y_{it}^{-}(\xi) + z^C_{it}(\xi) - z^D_{it}(\xi)\quad  \forall i, t &\\ 
    &R_{it}(\xi) \geq y^+_{it}(\xi) \quad \forall i ,t &\\
    &z^D_{it}(\xi) \le z_{it}(\xi) \quad \forall i, t &\\
    &z^C_{it}(\xi) \le K_i-z_{it}(\xi) \quad \forall i, t &\\
    &0 \leq z_{it}(\xi) \leq K_i \quad \forall i, t &\\
    &y^+_{it}(\xi) \leq M_1 \rho_{it}(\xi), \quad y^-_{it}(\xi) \leq M_1 (1 - \rho_{it}(\xi)) \quad \forall i, t &\\
    &y^-_{it}(\xi) \leq M_1 \delta_{it}(\xi), \quad z^C_{it}(\xi) \leq M_1 (1 - \delta_{it}(\xi)) \quad \forall i, t &\\
    &z^C_{it}(\xi) \leq M_1 \zeta_{it}(\xi), \quad z^D_{it}(\xi) \leq M_1 (1 - \zeta_{it}(\xi)) \quad \forall i, t &\\
    &&\\
    &e^+_{it}(\xi) = y^+_{it}(\xi) - d^{+}_{it}(\xi) &\\
    &e^-_{it}(\xi) = y^-_{it}(\xi) - d^{-}_{it}(\xi) &\\
    &e^C_{it}(\xi) = z^C_{it}(\xi) - \widehat{d^{C}_{it}}(\xi) + \widecheck{d^{C}_{it}}(\xi) &\\
    &\widehat{d^{C}_{it}}(\xi) \leq M_1 q^3_{it}(\xi), \quad \widecheck{d^{C}_{it}}(\xi) \leq M_1 (1 - q^3_{it}(\xi)) &\\
    &e^C_{it}(\xi) \leq K_i - z_{it}(\xi)&\\
    &e^D_{it}(\xi) = z^D_{it}(\xi) - \widehat{d^{D}_{it}}(\xi) + \widecheck{d^{D}_{it}}(\xi) &\\
    &\widehat{d^{D}_{it}}(\xi) \leq M_1 q^4_{it}(\xi), \quad \widecheck{d^{D}_{it}}(\xi) \leq M_1 (1 - q^4_{it}(\xi)) &\\
    &e^D_{it}(\xi) \leq z_{it}(\xi)&\\
    &e^{+}_{it}(\xi) \leq M_1 q^5_{it}(\xi), \quad e^{-}_{it}(\xi) \leq M_1 (1 - q^5_{it}(\xi)) &\\
    &e^{-}_{it}(\xi) \leq M_1 q^6_{it}(\xi), \quad e^{C}_{it}(\xi) \leq M_1 (1 - q^6_{it}(\xi)) &\\
    &e^{C}_{it}(\xi) \leq M_1 q^6_{it}(\xi), \quad e^{D}_{it}(\xi) \leq M_1 (1 - q^6_{it}(\xi)) &\\
    &&\\
    &z_{i,t+1}(\xi) = z_{it}(\xi) + e^C_{it}(\xi) - e^D_{it}(\xi) \quad \forall i, t &\\
    &\alpha_t = \sum_{i\in I}x_{it}, \quad \beta_t^+(\xi) = \sum_{i\in I}e^+_{it}(\xi), \quad \beta_t^-(\xi) = \sum_{i\in I}e^-_{it}(\xi)&\\
    &\gamma_t(\xi) = \sum_{i\in I}z_{it}(\xi), \quad \gamma^C_t(\xi) = \sum_{i\in I}e^C_{it}(\xi), \quad \gamma^D_t(\xi) = \sum_{i\in I}e^D_{it}(\xi)&\\
    &&\\
    & \sum_{i \in I} R_{it}(\xi) - \alpha_t = \beta^+_t(\xi) - \beta^-_t(\xi) + \gamma^C_t(\xi) - \gamma^D_t(\xi) \quad \forall t &\\
    &\sum_{i\in I}R_{it}(\xi) \geq \beta_{t}^{+}(\xi) \quad \forall t &\\ 
    &\gamma^D_t(\xi) \le \gamma_{t}(\xi) \quad \forall t &\\
    &\gamma^C_t(\xi) \le \sum_{i \in I}K_i - \gamma_{t}(\xi) \quad \forall t &\\
    &0 \leq \gamma_t(\xi) \leq \sum_{i \in I} K_i \quad \forall t &\\
    &\gamma_{t+1}(\xi) = \gamma_{t}(\xi) + \gamma^C_t(\xi) - \gamma^D_t(\xi) \quad \forall t &\\
    &\beta^+_t(\xi) \le M_2 \mu_t(\xi), \quad \beta^-_t(\xi) \le M_2 (1 - \mu_t(\xi)) \quad \forall t &\\ 
    &\beta^-_t(\xi) \le M_2 \eta_t(\xi), \quad \gamma^C_t(\xi) \le M_2 (1 - \eta_t(\xi))\quad \forall t &\\
    &\gamma^C_t(\xi) \le M_2\lambda_t(\xi), \quad \gamma^D_t(\xi) \le M_2(1 - \lambda_t(\xi)) \quad \forall t &\\
    &&\\
    &\sum_{i \in I}\widehat{d^{C}_{it}}(\xi) \leq \sum_{i \in I}y^-_{it}(\xi)&\\
    &\left(d^+_{it}(\xi) - \sum_{i \in I}y^-_{it}(\xi) \right) - \left(K_i - z_{it}(\xi)\right) \leq M_1(1-q^6_{it}(\xi))-\epsilon &\\
    &\left(K_i - z_{it}(\xi)\right) - e^C_{it}(\xi) \leq M_1 q^6_{it}(\xi)&\\
    &\left(K_i - z_{it}(\xi)\right) - \left(d^+_{it}(\xi) - \sum_{i \in I}y^-_{it}(\xi)\right) \leq M_1 (1-q^7_{it}(\xi))-\epsilon&\\
    & \left(e^C_{it}(\xi) \right) - \left( d^+_{it}(\xi) + z^c_{it}(\xi)\right) \leq M_1 q^7_{it}(\xi)&
    \end{align*}
\end{subequations}

\end{document}